MirrorCharge!/src/MirrorCharge/Java/JavaFunc.v
@@ -1,0 +1,355 @@
+Require Import Charge.Open.Subst.
+Require Import Charge.Open.Open.
+Require Import Charge.Open.Stack.
+Require Import Charge.Logics.BILogic.
+
+Require Import ExtLib.Core.RelDec.
+Require Import ExtLib.Data.Fun.
+Require Import ExtLib.Data.String.
+Require Import ExtLib.Tactics.Consider.
+
+Require Import MirrorCore.TypesI.
+Require Import MirrorCore.SymI.
+Require Import MirrorCore.Lambda.Expr.
+Require Import MirrorCore.syms.SymEnv.
+Require Import MirrorCore.syms.SymSum.
+
+Require Import Java.Logic.AssertionLogic.
+Require Import Java.Logic.SpecLogic.
+Require Import Java.Language.Lang.
+Require Import Java.Language.Program.
+Require Import Java.Semantics.OperationalSemantics.
+
+Require Import Coq.Strings.String.
+Require Import Coq.Bool.Bool.
+
+Require Import MirrorCharge.Java.JavaType.
+Require Import MirrorCharge.ModularFunc.ILogicFunc.
+Require Import MirrorCharge.ModularFunc.BILogicFunc.
+Require Import MirrorCharge.ModularFunc.LaterFunc.
+Require Import MirrorCharge.ModularFunc.BaseFunc.
+Require Import MirrorCharge.ModularFunc.ListFunc.
+Require Import MirrorCharge.ModularFunc.OpenFunc.
+Require Import MirrorCharge.ModularFunc.EmbedFunc.
+
+Set Implicit Arguments.
+Set Strict Implicit.
+
+Class JavaFunc func := {
+	fVar : var -> func;
+	fField : field -> func;
+	fClass : class -> func;
+	fVal : sval -> func;
+	fVarList : list var -> func;
+	fProg : Prog_wf -> func;
+	fCmd : cmd -> func;
+	fDExpr : dexpr -> func;
+	fFields : SS.t -> func;
+	fMethodSpec : func;
+	fProgEq : func;
+	fTriple : func;
+	fTypeOf : func;
+	fEval : func;
+	fFieldLookup : func;
+	fSetFold : typ -> func;
+	fSetFoldFun : func;
+	fPointsto : func;
+	fNull : func
+}.
+
+Section JavaFuncSum.
+	Context {func : Type} {H : JavaFunc func}.
+
+	Global Instance JavaFuncSumL (A : Type) : 
+		JavaFunc (func + A) := {
+			fVar v := inl (fVar v);
+			fField f := inl (fField f);
+			fClass c := inl (fClass c);
+			fVal v := inl (fVal v);
+			fVarList vs := inl (fVarList vs);
+			fProg P := inl (fProg P);
+			fCmd c := inl (fCmd c);
+			fDExpr e := inl (fDExpr e);
+			fFields fs := inl (fFields fs);
+			fMethodSpec := inl fMethodSpec;
+			fProgEq := inl fProgEq;
+			fTriple := inl fTriple;
+			fTypeOf := inl fTypeOf;
+			fEval := inl fEval;
+			fFieldLookup := inl fFieldLookup;
+			fSetFold t := inl (fSetFold t);
+			fSetFoldFun := inl fSetFoldFun;
+			fPointsto := inl fPointsto;
+			fNull := inl fNull
+		}.
+
+	Global Instance JavaFuncSumR (A : Type) : 
+		JavaFunc (A + func) := {
+			fVar v := inr (fVar v);
+			fField f := inr (fField f);
+			fClass c := inr (fClass c);
+			fVal v := inr (fVal v);
+			fVarList vs := inr (fVarList vs);
+			fProg P := inr (fProg P);
+			fCmd c := inr (fCmd c);
+			fDExpr e := inr (fDExpr e);
+			fFields fs := inr (fFields fs);
+			fMethodSpec := inr fMethodSpec;
+			fProgEq := inr fProgEq;
+			fTriple := inr fTriple;
+			fTypeOf := inr fTypeOf;
+			fEval := inr fEval;
+			fFieldLookup := inr fFieldLookup;
+			fSetFold t := inr (fSetFold t);
+			fSetFoldFun := inr fSetFoldFun;
+			fPointsto := inr fPointsto;
+			fNull := inr fNull
+		}.
+		
+	Global Instance JavaFuncExpr : 
+		JavaFunc (expr typ func) := {
+			fVar v := Inj (fVar v);
+			fField f := Inj (fField f);
+			fClass c := Inj (fClass c);
+			fVal v := Inj (fVal v);
+			fVarList vs := Inj (fVarList vs);
+			fProg P := Inj (fProg P);
+			fCmd c := Inj (fCmd c);
+			fDExpr e := Inj (fDExpr e);
+			fFields fs := Inj (fFields fs);
+			fMethodSpec := Inj fMethodSpec;
+			fProgEq := Inj fProgEq;
+			fTriple := Inj fTriple;
+			fTypeOf := Inj fTypeOf;
+			fEval := Inj fEval;
+			fFieldLookup := Inj fFieldLookup;
+			fSetFold t := Inj (fSetFold t);
+			fSetFoldFun := Inj fSetFoldFun;
+			fPointsto := Inj fPointsto;
+			fNull := Inj fNull
+		}.
+
+End JavaFuncSum.
+	
+Section JavaFuncInst.
+	Context {func : Type} {H : JavaFunc func}.
+
+	Inductive java_func :=
+	| pVar (_ : var)
+	| pField (_ : field)
+	| pClass (_ : class)
+	| pVal (_ : sval)
+	| pVarList (_ : list var) 
+	| pProg (_ : Prog_wf)
+	| pCmd (_ : cmd)
+	| pDExpr (_ : dexpr)
+	| pFields (_ : SS.t)
+	
+	| pMethodSpec
+	| pProgEq
+	| pTriple
+	| pTypeOf
+	| pEval
+	| pFieldLookup
+	
+	| pSetFold (_ : typ)
+	| pSetFoldFun 
+	
+	| pPointsto
+	| pNull.
+
+	Global Instance JavaFuncInst : JavaFunc java_func := {
+		fVar := pVar;
+		fField := pField;
+		fClass := pClass;
+		fVal := pVal;
+		fVarList := pVarList;
+		fProg := pProg;
+		fCmd := pCmd;
+		fDExpr := pDExpr;
+		fFields := pFields;
+		fMethodSpec := pMethodSpec;
+		fProgEq := pProgEq;
+		fTriple := pTriple;
+		fTypeOf := pTypeOf;
+		fEval := pEval;
+		fFieldLookup := pFieldLookup;
+		fSetFold := pSetFold;
+		fSetFoldFun := pSetFoldFun;
+		fPointsto := pPointsto;
+		fNull := pNull
+	}.
+
+	Fixpoint beq_list {A} (f : A -> A -> bool) (xs ys : list A) :=
+		match xs, ys with
+			| nil, nil => true
+			| x::xs, y :: ys => andb (f x y) (beq_list f xs ys)
+			| _, _ => false
+		end.
+
+	Definition typeof_java_func bf :=
+		match bf with
+		    | pVar _ => Some tyVar
+		    | pField _ => Some tyField
+		    | pClass _ => Some tyClass
+		    | pVal _ => Some tyVal
+		    | pVarList _ => Some tyVarList
+		    | pProg _ => Some tyProg
+		    | pCmd _ => Some tyCmd
+		    | pDExpr _ => Some tyDExpr
+		    | pFields _ => Some tyFields
+		
+		    | pMethodSpec => Some (tyArr tyClass (tyArr tyString (tyArr tyVarList
+		    	 (tyArr tyVar (tyArr tySasn (tyArr tySasn tySpec))))))
+		    | pProgEq => Some (tyArr tyProg tySpec)
+		    | pTriple => Some (tyArr tySasn (tyArr tySasn (tyArr tyCmd tySpec)))
+		    | pEval => Some (tyArr tyDExpr tyExpr)
+		    
+		    | pTypeOf => Some (tyArr tyVar (tyArr tyVal tyProp))
+		    
+		    | pFieldLookup => Some (tyArr tyProg (tyArr tyClass (tyArr tyFields tyProp)))
+		    
+		    | pSetFoldFun => Some (tyArr tyString (tyArr tyString (tyArr tySasn tySasn)))
+		    | pSetFold t => Some (tyArr (tyArr tyString (tyArr t t)) (tyArr tyFields (tyArr t t)))
+		    
+		    | pPointsto => Some (tyArr tyVal (tyArr tyField (tyArr tyVal tyAsn)))
+		    
+		    | pNull => Some tyVal
+		end.
+
+	Definition java_func_eq (a b : java_func) : option bool :=
+	  match a , b with
+	    | pVar a, pVar b => Some (a ?[ eq ] b)
+	    | pField a, pField b => Some (a ?[ eq ] b)
+	    | pClass a, pClass b => Some (a ?[ eq ] b)
+		| pVal a, pVal b => Some (beq_val a b)
+	    | pVarList a, pVarList b => Some (beq_list beq_string a b)
+	    | pProg a, pProg b => Some true (* THIS IS FALSE! We need an equivalence checker for programs. This should just be syntactic equality. *)
+	    | pCmd a, pCmd b => Some (beq_cmd a b)
+	    | pDExpr e1, pDExpr e2 => Some (beq_dexpr e1 e2)
+	    | pFields a, pFields b => Some (SS.equal a b)
+	        
+	    | pMethodSpec, pMethodSpec => Some true
+	    | pProgEq, pProgEq => Some true
+		| pTriple, pTriple => Some true
+	
+	    | pTypeOf, pTypeOf => Some true
+	
+		| pEval, pEval => Some true
+	
+	    | pPointsto, pPointsto => Some true
+	    | pFieldLookup, pFieldLookup => Some true
+	    | pSetFold t, pSetFold u => Some (t ?[ eq ] u)
+	    | pSetFoldFun, pSetFoldFun => Some true
+	
+	    | pNull, pNull => Some true
+	    | _, _ => None
+	  end.
+
+    Global Instance RelDec_java_func : RelDec (@eq java_func) := {
+      rel_dec a b := match java_func_eq a b with 
+    	  		       | Some b => b 
+    		 	       | None => false 
+    			     end
+    }.
+
+    Global Instance RelDec_Correct_ilfunc : RelDec_Correct RelDec_java_func.
+    Proof.
+      constructor.
+      destruct x; destruct y; simpl;
+      try solve [ try rewrite Bool.andb_true_iff ;
+                  repeat rewrite rel_dec_correct; intuition congruence ];
+                  	admit.
+    Qed.
+  
+Definition set_fold_fun (x : String.string) (f : field) (P : sasn) :=
+	(`pointsto) (x/V) `f `null ** P.
+  
+  	 Definition java_func_symD bf :=
+		match bf as bf return match typeof_java_func bf with
+								| Some t => typD t
+								| None => unit
+							  end with
+              | pVar v => v
+              | pClass c => c
+              | pField f => f
+              | pProg p => p
+              | pVal v => v
+              | pVarList vs => vs
+              | pCmd c => c
+              | pDExpr e => e
+              | pFields fs => fs
+
+              | pMethodSpec => method_spec
+              | pProgEq => prog_eq
+              | pTriple => triple
+              | pEval => eval
+              
+              | pTypeOf => typeof
+                            
+              | pFieldLookup => field_lookup
+              | pSetFold t => @SS.fold (typD t)
+              | pSetFoldFun => set_fold_fun
+              
+              | pPointsto => pointsto
+              
+              | pNull => null
+	end.
+
+	Global Instance RSym_BaseFunc : SymI.RSym java_func := {
+	  typeof_sym := typeof_java_func;
+	  symD := java_func_symD;
+	  sym_eqb := java_func_eq
+	}.
+
+	Global Instance RSymOk_BaseFunc : SymI.RSymOk RSym_BaseFunc.
+	Proof.
+		admit.
+
+		(*
+		split; intros.
+		destruct a, b; simpl; try apply I.
+		+ consider (v ?[ eq ] v0); intuition congruence.
+		+ consider (f ?[ eq ] f0); intuition congruence.
+		+ consider (c ?[ eq ] c0); intuition congruence.
+		+ consider (t ?[ eq ] t0); intuition congruence.
+		+ consider (t ?[ eq ] t1 && t0 ?[ eq ] t2)%bool; 
+		  intuition congruence.
+*)
+	Qed.
+
+End JavaFuncInst.
+
+Section MakeJavaFunc.
+	Context {func : Type} {H : JavaFunc func} {HT : ListFunc typ func}.
+
+	Definition mkTriple P c Q := App (App (App fTriple P) Q) c.
+	Definition mkFieldLookup P C f := App (App (App fFieldLookup P) C) f.
+	Definition mkSetFold t x f P:= (App (App (App (fSetFold t) (App fSetFoldFun x)) f) P). 
+	Definition mkTypeOf C x := App (App fTypeOf C) x.
+	Definition mkVal v : expr typ func := Inj (fVal v).
+	Definition mkField f : expr typ func := Inj (fField f).
+	Definition mkVar f : expr typ func := Inj (fVar f).
+	Definition mkClass c : expr typ func := Inj (fClass c).
+	Definition mkVarList vs : expr typ func := Inj (fVarList vs).
+	Definition mkProg P : expr typ func := Inj (fProg P).
+	Definition mkCmd c : expr typ func := Inj (fCmd c).
+	Definition mkDExpr e : expr typ func := Inj (fDExpr e).
+	Definition mkFields fs : expr typ func := Inj (fFields fs).
+	Definition mkProgEq P := App fProgEq P.
+	
+	Definition mkExprList es :=
+		(fold_right (fun (e : dexpr) (acc : expr typ func) => 
+			mkCons tyExpr (mkDExpr e) acc) (mkNil tyExpr) es).
+	
+	Definition mkEval e s := App (App fEval e) s.
+	
+	Definition mkNull : expr typ func := fNull.
+
+End MakeJavaFunc.
+
+Definition func := (SymEnv.func + java_func + @ilfunc typ + @bilfunc typ + 
+                    @base_func typ + @list_func typ + @open_func typ + 
+                    @embed_func typ + @later_func typ)%type.
+
+
